# Exercise 6: Automating Natural Deduction

1. Consider the following rule based system:
    - i) $F\implies D$
    - ii) $F\implies G$
    - iii) $E\implies D$
    - iv) $B\implies E$
    - v) $E\implies A$
    - vi) $C\implies A$
    - vii) $G\implies C$
    - viii) $G\implies B$
    - ix) $D\implies B$

a) Given $F$, prove $E$ by forward and backward chaining.
b) Given $G$, prove $D$ by forward and backward chaining.
c) Given $D$, prove $A$ by forward and backward chaining.


```{dropdown} **Solution**

a)
* Forward chaining
    - Given $F$, by (i) $D$ must be True.
    - Given $D$, by (ix) $B$ must be True.
    - Given $B$, by (iv) $E$ must be True and the proof is complete.
* Backward Chaining
    - Assume $E$, by (iv) obtain new goal $B$.
    - Goal $B$ leads to new goal $D$ by (xi).
    - Goal $D$ leads to new goal $F$ by (i).
    - $F$ is known and so the proof is complete.

b)
* Forward Chaining
    - Given $G$, by (viii) $B$ is True.
    - Given $B$, by (iv) $E$ is True.
    - Given $E$, by (iii) $D$ is True and and the proof is complete.
* Backward Chaining
    - Assume $D$, obtain new goal $E$ by (iii).
    - Goal $E$ leads to new goal $B$ by (iv).
    - Goal $B$ leads to new goal $G$ by (xiii).
    - $G$ is known and so the proof is complete.

c)
* Forward Chaining
    - Given $D$, by (ix) $B$ is True.
    - Given $B$, by (iv) $E$ is True.
    - Given $E$, by (v) $A$ is True and the proof is complete.
* Backward Chaining
    - Assuming $A$, new goal $E$ by (v)
    - Assuming $E$, new goal $B$ by (iv)
    - Assuming $B$, new goal $D$ by (ix)
    - $D$ is known and the proof is complete.
```

2. Consider the following rule based system:
    - i) $D\implies A$
    - ii) $D\implies E$
    - iii) $E\implies F$
    - iv) $D\implies C$
    - v) $C\implies F$
    - vi) $F\implies B$
    - vii) $B\implies C$
    - viii) $A\implies G$
    - ix) $G\implies B$

a) Given $E$, prove $C$ by forward and backward chaining.
b) Given $G$, prove $F$ by forward and backward chaining.
c) Given $A$, prove $B$ by forward and backward chaining.

```{dropdown} **Solution**
a)
* Forward Chaining
    - Given $E$, by (iii) $F$ is True.
    - Given $F$, by (vi) $B$ is True.
    - Given $B$, by (vii) $C$ is True and the proof is complete.
* Backward Chaining
    - Assume $C$, new goal $B$ by (vii).
    - Assume $B$, new goal $F$ by (iv).
    - Assume $F$, new goal $E$ by (iii).
    - $F$ is known and the proof is complete.

b)
* Forward Chaining
    - Given $G$, by (ix) $B$ is True.
    - Given $B$, by (vii) $C$ is True.
    - Given $C$, by (v) $F$ is True and the proof is complete.
* Backward Chaining
    - Assume $F$, new goal $C$ by (v).
    - Assume $C$, new goal $B$ by (vii).
    - Assume $B$, new goal $G$ by (ix).
    - $G$ is known and the proof is complete.

c)
    - Given $A$, by (viii) $G$ is True.
    - Given $G$, by (ix) $B$ is True and the proof is complete.
* Backward Chaining
    - Assume $B$, new goal $G$ by (ix).
    - Assume $G$, new goal $A$ by (viii).
    - $A$ is known and the proof is complete.

```

3. Consider the following rule based system:
    - i) $D\implies B$
    - ii) $D\implies G$
    - iii) $C\implies G$
    - iv) $C\implies A$
    - v) $G\implies E$
    - vi) $D\implies B$
    - vii) $B\implies F$
    - viii) $E\implies F$
    - ix) $F\implies H$
    - x) $E\implies A$
    - xi) $A\implies I$
    - xii) $H\implies I$

a) Given $G$, prove $I$ by forward and backward chaining.
b) Given $C$, prove $H$ by forward and backward chaining.
c) Given $D$, prove $A$ by forward and backward chaining.

```{dropdown} **Solution**
a)
* Forward Chaining
    - Given $G$, by (v) $E$ is True.
    - Given $E$, by (x) $A$ is True.
    - Given $A$, by (xi) $I$ is True and the proof is complete.
* Backward Chaining
    - Assume $I$, new goal $A$ by (xi).
    - Assume $A$, new goal $E$ by (x).
    - Assume $E$, new goal $G$ by (v).
    - $G$ is known and the proof is complete.

b)
* Forward Chaining
    - Given $C$, by (iii) $G$ is True.
    - Given $G$, by (v) $E$ is True.
    - Given $E$, by (viii) $F$ is True.
    - Given $F$, by (ix) $H$ is True and the proof is complete.
* Backward Chaining
    - Assume $H$, new goal $F$ by (ix).
    - Assume $F$, new goal $E$ by (viii).
    - Assume $E$, new goal $G$ by (v).
    - Assume $G$, new goal $C$ by (iii).
    - $C$ is known and the proof is complete.

c)
    - Given $D$, by (ii) $G$ is True.
    - Given $G$, by (v) $E$ is True.
    - Given $E$, by (x) $A$ is True and the proof is complete.
* Backward Chaining
    - Assume $A$, new goal $E$ by (x).
    - Assume $E$, new goal $G$ by (v).
    - Assume $G$, new goal $D$ by (ii).
    - $D$ is known and the proof is complete.

```