# Exercise 4: Natural Deduction

1. Prove the argument $P\implies Q\land R,\ R\implies S,\ P,\ Q\ :\ S$

```{dropdown} **Solution**   
| Step |                                    | Rule | Premises |
|-----:|:-----------------------------------|:-----|-------------:|
| 1.   | $P\implies Q$                       | Premise | {1}|
| 2.   | $P$                                | Premise | {2}|
| 3.   | $Q\land R$                         | Modus Ponens $_{1,2}$ | {1,2}|
| 4.   | $Q$                                | Premise | {4} |
| 5.   | $R$                                | $\land$-elimination $_{3,4}$ | {1,2,4}|
| 6.   | $R\implies S$                      | Premise | {6}|
| 7.   | $S$                                | Modus Ponens $_{5,6}$ | {1,2,4,6}|
```

2. Prove the argument $\lnot P\implies \lnot Q,\ Q,\ P\implies S\land Q\ :\ S $

```{dropdown} **Solution**   
| Step |                                    | Rule | Premises |
|-----:|:-----------------------------------|:-----|-------------:|
| 1.   | $\lnot P\implies \lnot Q$          | Premise | {1}|
| 2.   | $Q$                                | Premise | {2}|
| 3.   | $P$                                | Modus Tollens $_{1,2}$ | {1,2}|
| 4.   | $P\implies Q\land S$               | Premise | {4} |
| 5.   | $Q\land S$                         | Modus Ponens $_{3,4}$ | {1,2,4}|
| 6.   | $S$                                | $\land$-elimination $_{5}$ | {1,2,4}|
```

3. Prove that the following argument is invalid by showing that there is a contradiction: $\lnot(P\land Q)\implies S,\ \lnot S,\ P\implies\lnot Q\ :\ \lnot Q$

```{dropdown} **Solution**   
| Step |                                    | Rule | Premises |
|-----:|:-----------------------------------|:-----|-------------:|
| 1.   | $\lnot (P\land Q)\implies S$       | Premise | {1}|
| 2.   | $\lnot S$                          | Premise | {2}|
| 3.   | $P\land Q$                         | Modus Tollens $_{1,2}$ | {1,2}|
| 4.   | $P$                                | $\land$-elimination $_3$ | {1,2} |
| 5.   | $Q$                                | $\land$-elimination $_3$ | {1,2} |
| 6.   | $P\implies \lnot Q$                | Premise | {6}|
| 7.   | $\lnot Q$                          | Modus Ponens $_{4,6}$ | {1,2,6}|

We have been able to derive the conlusion and its negation - a contradiction. The argument therefore cannot be valid.
```

4. Prove the argument $(P\land Q)\implies R,\ \lnot R,\ P,\ :\ \lnot Q$

```{dropdown} **Solution**   
| Step |                                    | Rule | Premises |
|-----:|:-----------------------------------|:-----|-------------:|
| 1.   | $(P\land Q)\implies R$             | Premise | {1}|
| 2.   | $\lnot R$                          | Premise | {2}|
| 3.   | $\lnot(P\land Q)$                  | Modus Tollens $_{1,2}$ | {1,2}|
| 4.   | $P$                                | Premise | {4} |
| 5.   | $\lnot Q$                          | $\land$-elimination $_{3,4}$ | {1,2,4}|
```

5. Prove that the following argument is invalid by showing that there is a contradiction: $P\iff Q,\ P,\ Q\implies\lnot R,\ R\ :\ Q$

```{dropdown} **Solution**   
| Step |                                    | Rule | Premises |
|-----:|:-----------------------------------|:-----|-------------:|
| 1.   | $P\iff Q$                          | Premise | {1}|
| 2.   | $P$                                | Premise | {2}|
| 3.   | $P\implies Q$                                | Biconditional elimination $_{1,2}$ | {1,2}|
| 4.   | $Q$                                | Modus Ponens $_{2,3}$ | {1,2} |
| 4.   | $Q\implies\lnot R$                 | Premise | {5} |
| 5.   | $R$                                | Premise | {6}|
| 6.   | $\lnot Q$                          | Modus Tollens $_{5,6}$ | {5,6} |

We have been able to derive the conlusion and its negation - a contradiction. The argument therefore cannot be valid.
```

## Stretchers

The following problems use rules we have not specifically introduced and require an element of lateral thinking.

6. Prove the argument $P\implies Q,\ \lnot Q\ :\ P\implies R$

You may find the following equivalence helpful: $A\implies B \equiv \lnot A \lor B$.

```{dropdown} **Solution**   
| Step |                                    | Rule | Premises |
|-----:|:-----------------------------------|:-----|-------------:|
| 1.   | $P\implies Q$                      | Premise | {1}|
| 2.   | $\lnot Q$                          | Premise | {2}|
| 3.   | $\lnot P$                          | Modus Ponens $_{1,2}$ | {1,2}|
| 4.   | $\lnot P \lor R$                   | $\lor$-Introduction $_3} | {1,2} |
| 5.   | $P\implies R$                      | Equivalence $_{4}$ | {1,2}|
```

7. Prove the argument $P\land Q,\ Q\implies\lnot R\ :\ \lnot(R\land\lnot S)$

```{dropdown} **Solution**   
| Step |                                    | Rule | Premises |
|-----:|:-----------------------------------|:-----|-------------:|
| 1.   | $P\land Q$                         | Premise | {1}|
| 2.   | $Q$                                | $\land$-elimination $_1$ | {1}|
| 3.   | $Q\implies\lnot R$                 | Premise  | {2}|
| 4.   | $\lnot R$                         | Modus Ponens $_{2,3}$ | {1,2} |
| 5.   | $\lnot R \lor S$                   |  $\lor$-Introduction $_4$ | {1,2} |
| 6.   | $\lnot(R\land\lnot S)$             | de Morgan $_{5}$ | {1,2}|
```

8. Prove the argument $\lnot P,\ \lnot Q\ :\ P\iff Q$

```{dropdown} **Solution**   
| Step |                                    | Rule | Premises |
|-----:|:-----------------------------------|:-----|-------------:|
| 1.   | $\lnot P$                          | Premise | {1}|
| 2.   | $\lnot P \lor Q$                   | $\lor$-Introduction $_1$ | {1} |
| 3.   | $P\implies Q$                      | Equivalence $_{2}$ | {1}|
| 4.   | $\lnot Q$                          | Premise | {2} |
| 5.   | $\lnot Q\lor P$                    | $\lor$-Introduction $_4$ | {2} |
| 6.   | $Q\implies P$                      | Equivalence $_{5}$ | {2}|
| 7.   | $(P\implies Q)\land(Q\implies P)$  | $\land$-Introduction_{3,6}$ | {1,2}|
| 8.   | $P\iff Q$                          | Equivalence $_{7}$ | {1,2}|
```

9. Prove the argument $P\implies \lnot Q \land\lnot R,\ P,\ :\ \lnot Q$

```{dropdown} **Solution**   
| Step |                                    | Rule | Premises |
|-----:|:-----------------------------------|:-----|-------------:|
| 1.   | $P\implies \lnot Q \land\lnot R)$  | Premise | {1}|
| 2.   | $P$                                | Premise | {2}|
| 3.   | $\lnot Q\land \lnot RQ$            | Modus Ponens $_{1,2}$ | {1,2}|
| 4.   | $\lnot(Q\lor R)$                    | de Morgam $_{3}$ | {1,2} |
| 5.   | $\lnot Q$                          | Modus Tollendo Ponens $_{4}$ | {1,2}|
```